LTS.thy
@@ -1,0 +1,88 @@
+theory LTS
+
+imports Main
+
+begin
+
+section {* Labelled transition systems *}
+
+text {* The semantics of a B component is a discrete, eventful, state-transition systems. We 
+first define what is meant exactly by such systems. Any system is, at a given time in a state. 
+Conversely, a system has a set of possible states. A system evolves from state to state,
+and such changes called transitions. Also when a system makes a transition, this is observable
+and this observation is called an event. State, transition and event are three different
+entities and a type is declared for each: *}
+
+typedecl STATE
+typedecl TRANSITION
+typedecl EVENT
+
+text {* These different entities are related through the following functions: *}
+consts src :: "TRANSITION \<Rightarrow> STATE"
+consts dst :: "TRANSITION \<Rightarrow> STATE"
+consts evt :: "TRANSITION \<Rightarrow> EVENT"
+
+record LTS =
+  init :: "STATE set" (* a set of initial states *)
+  trans :: "TRANSITION set" (* a set of transitions *)
+  
+inductive_set states :: "LTS \<Rightarrow> STATE set" for m :: LTS where
+  base[elim!]: "s \<in> init m \<Longrightarrow> s \<in> states m"
+| step[elim!]: "\<lbrakk> t \<in> trans m; src t \<in> states m \<rbrakk> \<Longrightarrow> dst t \<in> states m"
+  
+definition successors :: "LTS \<Rightarrow> STATE set \<Rightarrow> STATE set" where
+"successors lts S \<equiv> { s | s . \<exists> t \<in> trans lts. src t \<in> S \<and> dst t = s}"
+  
+text {* A few lemmas related to reachable states are then enunciated and proved. 
+First, all the initial states are reachable states:*}
+
+lemma reachable_init: "init m \<subseteq> states m" 
+  by auto
+
+lemma reachable_stable: "successors m (states m) \<subseteq> states m"
+  unfolding successors_def by auto
+  
+text {* The following lemma is related to the identification of sufficient conditions to establish 
+safety properties. Consider a property that is satisfied by some set of states $S$. If the initial 
+states are in $S$, and if the successors of $S$ are in $S$ then all the reachable states are in 
+$S$. *}
+
+lemma reachable_induct_set:
+  assumes base: "init m \<subseteq> S" and step: "successors m S \<subseteq> S"
+  shows "(states m) \<subseteq> S"
+proof
+  fix x
+  assume "x \<in> states m"
+  thus "x \<in> S"
+  proof (induct x)
+    fix i
+    assume "i \<in> init m"
+    with base show "i \<in> S" ..
+  next
+    fix t
+    assume "t \<in> trans m" "src t \<in> states m" "src t \<in> S"
+    with step show "dst t \<in> S" unfolding successors_def by auto
+  qed
+qed
+
+text {* Next we enunciate and prove a similar lemma for predicates. *}
+lemma reachable_induct_predicate:
+  assumes base: "\<forall> s \<in> init m . p s" and 
+          step: "\<forall> t \<in> trans m . p (src t) \<longrightarrow> p (dst t)"
+  shows "\<forall> s \<in> (states m) . p s"
+proof
+  fix x
+  assume "x \<in> states m" 
+  thus "p x"
+  proof (induct x)
+    fix i
+    assume "i \<in> init m"
+    with base show "p i" ..
+  next
+    fix t
+    assume "t \<in> trans m" "src t \<in> states m" "p (src t)"
+    with step show "p (dst t)" unfolding successors_def by auto
+  qed
+qed
+
+end
