Simulation.thy
@@ -1,0 +1,76 @@
+theory Simulation
+
+imports Main LTS
+
+begin
+section {* Behaviour: a set of traces *}
+
+text {* We introduce the notion of simulation: a relation between the states of one LTS
+and the states of another LTS such that any transition taken by the former can be simulated
+by the latter, i.e. the latter can follow a transition that is labeled with the same event,
+and leads to a state where it can continue the simulation: *}
+
+definition lts_simulation_init :: "STATE rel \<Rightarrow> LTS \<Rightarrow> LTS \<Rightarrow> bool" where
+  "lts_simulation_init r l1 l2 \<equiv> \<forall> s1 \<in> init l1 . \<exists> s2 \<in> init l2 . (s1, s2) \<in> r"
+
+definition lts_simulation_transition :: "STATE rel \<Rightarrow> LTS \<Rightarrow> LTS \<Rightarrow> bool" where
+  "lts_simulation_transition r l1 l2 \<equiv> 
+    \<forall> s1 \<in> states l1 . \<forall> s2 \<in> states l2 . (s1, s2) \<in> r \<longrightarrow>
+      (\<forall> t1 \<in> trans l1 . src t1 = s1 \<longrightarrow>
+        (\<exists> t2 \<in> trans l2 . (src t2 = s2 \<and> evt t1 = evt t2 \<and> (dst t1, dst t2) \<in> r)))"
+
+definition lts_simulation :: "STATE rel \<Rightarrow> LTS \<Rightarrow> LTS \<Rightarrow> bool" where
+  "lts_simulation r l1 l2 \<equiv> lts_simulation_init r l1 l2 \<and> lts_simulation_transition r l1 l2"
+
+text {* Let us verify some basic properties of simulations. First we have that the
+identity relation establishes that a LTS simulates itself. *}
+  (* maybe use Id_on (states l) instead of Id ? *)
+lemma lts_simulation_identity :
+  "lts_simulation Id l l" unfolding lts_simulation_def
+proof
+  show "lts_simulation_init Id l l" unfolding lts_simulation_init_def Id_def by auto
+next
+  show "lts_simulation_transition Id l l" unfolding lts_simulation_transition_def Id_def by auto
+qed
+
+text {* Second, we have that the composition of two simulation relations 
+is a simulation relation. *}
+lemma lts_simulation_transitivity:
+  "lts_simulation r12 l1 l2 \<and> lts_simulation r23 l2 l3 \<Longrightarrow> lts_simulation (r23 O r12) l1 l3"
+  unfolding lts_simulation_def lts_simulation_init_def lts_simulation_transition_def relcomp_def 
+sorry
+
+text {* Next we carry these properties over to the simulates relation over LTS. *}
+
+text {* Based on the notion of simulation, we introduce the relation simulates on LTS: *}
+definition lts_simulates :: "LTS \<Rightarrow> LTS \<Rightarrow> bool" (infixl "\<sim>" 50) where
+  "(l1 \<sim> l2) \<equiv> \<exists> r . lts_simulation r l2 l1"
+
+lemma lts_simulates_reflexivity: "l \<sim> l" 
+  unfolding lts_simulates_def
+proof
+  show "lts_simulation Id l l" by (rule lts_simulation_identity)
+qed
+
+lemma lts_simulates_transitivity:
+assumes
+  s12: "l1 \<sim> l2" and s23: "l2 \<sim> l3"
+shows
+  "l1 \<sim> l3"
+unfolding lts_simulates_def
+sorry
+
+(*
+proof
+  from s12 obtain r where "lts_simulation r l2 l1" unfolding lts_simulates_def ..
+moreover
+  from s23 obtain s where "lts_simulation s l3 l2" unfolding lts_simulates_def ..
+ultimately
+  obtain x where "x = r O s"
+    sorry
+  from this show "lts_simulation x l3 l1"
+    sorry
+qed
+*)
+  
+end
